ADTExamples/MinPlusMax.v
@@ -1,6 +1,7 @@
 Require Import Common String ADT ADTRefinement.Specs.
 Require Import ADTRefinement ADTCache ADTRepInv Pick ADTHide DelegateMethods.
-Require Import ADTExamples.BinaryOperationSpec ADTExamples.CombineBinaryOperationsSpec.
+Require Import ADTExamples.BinaryOperationSpec ADTExamples.CombineBinaryOperationsSpec
+        ADTRefinement.BuildADTRefinements ADTRefinement.BuildADTSetoidMorphisms.
 
 Section MinMaxExample.
 
@@ -13,7 +14,7 @@ Section MinMaxExample.
 
   Definition defaultSpec : nat -> Prop := fun _ => True.
 
-  Definition MinMaxSpec 
+  Definition MinMaxSpec
   : ADT MinMaxSig :=
     ADTRep multiset `[
              def "Insert" `[ m `: rep , n `: nat ]` : rep :=
@@ -27,8 +28,20 @@ Section MinMaxExample.
   Variable MinMaxImpl : ADT MinMaxSig.
   Variable refineMinMax : refineADT MinMaxSpec MinMaxImpl.
 
-  Definition foo idx : 
-    fst (ObserverDomCod (CombTwoOpCollectionSig "MinPlusMax") idx) -> 
+  Lemma extract_MinMaxSiR :
+    exists SiR : multiset -> Rep MinMaxImpl -> Prop,
+      (forall idx : ObserverIndex MinMaxSig,
+         refineObserver SiR (ObserverMethods MinMaxSpec idx)
+                        (ObserverMethods MinMaxImpl idx)) /\
+            (forall idx : MutatorIndex MinMaxSig,
+               refineMutator SiR (MutatorMethods MinMaxSpec idx)
+                             (MutatorMethods MinMaxImpl idx)).
+  Proof.
+    inversion refineMinMax; subst; eauto.
+  Defined.
+
+  Definition foo idx :
+    fst (ObserverDomCod (CombTwoOpCollectionSig "MinPlusMax") idx) ->
     nat.
   Proof.
     destruct idx; inversion s_bounded.
@@ -40,8 +53,8 @@ Section MinMaxExample.
     eauto.
   Defined.
 
-  Definition bar idx : 
-    nat -> 
+  Definition bar idx :
+    nat ->
     snd (ObserverDomCod (CombTwoOpCollectionSig "MinPlusMax") idx).
   Proof.
     destruct idx; inversion s_bounded.
@@ -53,14 +66,152 @@ Section MinMaxExample.
     eauto.
   Defined.
 
+  Definition delegateADTSiR (or : multiset) (nr : multiset * Rep MinMaxImpl) := 
+    or = fst nr.
+
+  Ltac autorefine :=
+    unfold repInvSiR in *|-*;
+    subst; split_and; intros;
+    autorewrite with refine_monad;
+    eauto 50 with cache_refinements typeclass_instances;
+    match goal with
+        |- refine _ (ret _) => let v := fresh in
+                               let CompV := fresh in
+                               intros v CompV; apply computes_to_inv in CompV;
+                               subst; econstructor; intros; eauto
+      | _ => idtac
+    end.
+
+  Tactic Notation "hone''" "observer" constr(obsIdx) "using" constr(obsBod) :=
+    let A :=
+        match goal with
+            |- Sharpened ?A => constr:(A) end in
+    let ASig := match type of A with
+                    ADT ?Sig => Sig
+                end in
+    let mutSigs :=
+        match ASig with
+            BuildADTSig ?mutSigs _ => constr:(mutSigs) end in
+    let obsSigs :=
+        match ASig with
+            BuildADTSig _ ?obsSigs => constr:(obsSigs) end in
+    let mutDefs :=
+        match A with
+            BuildADT ?mutDefs _  => constr:(mutDefs) end in
+    let obsDefs :=
+        match A with
+            BuildADT _ ?obsDefs  => constr:(obsDefs) end in
+    let Rep' :=
+        match A with
+            @BuildADT ?Rep _ _ _ _ => constr:(Rep) end in
+    let MutatorIndex' := eval simpl in (MutatorIndex ASig) in
+    let ObserverIndex' := eval simpl in (ObserverIndex ASig) in
+    let ObserverDomCod' := eval simpl in (ObserverDomCod ASig) in
+    let obsIdxB := eval simpl in
+    (@Build_BoundedString (List.map obsID obsSigs) obsIdx _) in
+      apply SharpenStep with
+      (adt' := ADTReplaceObsDef mutDefs obsDefs obsIdxB 
+                                (@Build_obsDef Rep'
+                                               {| obsID := obsIdx;
+                                                  obsDom := fst (ObserverDomCod' obsIdxB);
+                                                  obsCod := snd (ObserverDomCod' obsIdxB)
+                                               |}
+                                               obsBod
+                                )); cbv beta in *; simpl in * .
+
+  Tactic Notation "hone''" "mutator" constr(mutIdx) "using" constr(mutBod) :=
+    let A :=
+        match goal with
+            |- Sharpened ?A => constr:(A) end in
+    let ASig := match type of A with
+                    ADT ?Sig => Sig
+                end in
+    let mutSigs :=
+        match ASig with
+            BuildADTSig ?mutSigs _ => constr:(mutSigs) end in
+    let obsSigs :=
+        match ASig with
+            BuildADTSig _ ?obsSigs => constr:(obsSigs) end in
+    let mutDefs :=
+        match A with
+            BuildADT ?mutDefs _  => constr:(mutDefs) end in
+    let obsDefs :=
+        match A with
+            BuildADT _ ?obsDefs  => constr:(obsDefs) end in
+    let Rep' :=
+        match A with
+            @BuildADT ?Rep _ _ _ _ => constr:(Rep) end in
+    let MutatorIndex' := eval simpl in (MutatorIndex ASig) in
+    let ObserverIndex' := eval simpl in (ObserverIndex ASig) in
+    let MutatorDom' := eval simpl in (MutatorDom ASig) in
+    let mutIdxB := eval simpl in
+    (@Build_BoundedString (List.map mutID mutSigs) mutIdx _) in
+        apply SharpenStep with
+        (adt' := ADTReplaceMutDef mutDefs obsDefs mutIdxB 
+                                  (@Build_mutDef Rep'
+                                                 {| mutID := mutIdx;
+                                                    mutDom := MutatorDom' mutIdxB
+                                                 |}
+                                                 mutBod
+                                )); cbv beta in *; simpl in * .
+
+  Arguments delegateADTSiR or nr / .
+
   Definition MinPlusMaxImpl (defaultValue : nat)
   : Sharpened MinPlusMaxSpec.
   Proof.
-    eapply SharpenStep.
-    eapply refineADT_DelegatedMethods with 
-    (delegateDomCod := ObserverDomCod MinMaxSig)
-    (delegateADT := MinMaxImpl).
-    eapply SharpenStep with (adt' := 
+    (* Add a MinMax instance to the representation so we can delegate to it. *)
+    hone' representation using delegateADTSiR.
+    (* Implement the Insert Mutator.  *)
+    hone'' mutator "Insert"%string using 
+          (fun r x =>
+           r1 <- MutatorMethods MinPlusMaxSpec {| bounded_s := "Insert"%string |} (fst r) x;
+           r2 <- MutatorMethods MinMaxImpl {|bounded_s := "Insert"%string |} (snd r) x;
+           ret (r1, r2)).
+    destruct extract_MinMaxSiR as [MinMaxSiR [refineMinMaxObs refineMinMaxMut] ].
+    eapply refineADT_BuildADT_Rep with
+    (SiR := fun (or nr : Rep MinPlusMaxSpec * Rep MinMaxImpl) =>
+              or = nr /\
+              MinMaxSiR (fst nr) (snd nr)).
+    unfold getMutDef; simpl; unfold ith_obligation_2; simpl.
+    intros mutIdx r_o r_n; find_if_inside; intros; intuition;
+    subst; simpl; autorefine.
+    unfold refine; intros; inversion_by computes_to_inv; subst;
+    econstructor.
+    econstructor; intros; subst; eexists; split.
+    econstructor; eauto.
+    instantiate (1 := (x, x0)); reflexivity.
+    econstructor; split; eauto.
+    generalize (refineMinMaxMut {| bounded_s := "Insert"%string |} _ _ n H1 _ H2);
+    simpl; unfold getMutDef; simpl; intros.
+    inversion_by computes_to_inv; unfold add_spec in *.
+      assert (x1 = x) by
+          (apply functional_extensionality;
+           intros; rewrite H0, H3; reflexivity).
+      rewrite H in H4; assumption.
+      intros; unfold refineObserver; intros; intuition; subst; 
+      reflexivity. 
+    (* Implement the MinPlusMax Observer. *)
+      unfold getMutDef; simpl.
+      unfold two_op_spec.
+    hone'' observer "MinPlusMax"%string using 
+           (fun (r : Rep MinPlusMaxSpec * Rep MinMaxImpl)
+                n =>
+              (min <- (ObserverMethods MinMaxImpl
+                                       {|bounded_s := "Min"%string |} (snd r) n);
+               max <- (ObserverMethods MinMaxImpl
+                                       {|bounded_s := "Max"%string |} (snd r) n);
+               ret ((min + max)))%comp).
+    destruct extract_MinMaxSiR as [MinMaxSiR [refineMinMaxObs refineMinMaxMut] ].
+    eapply refineADT_BuildADT_Rep with
+    (SiR := fun (or nr : Rep MinPlusMaxSpec * Rep MinMaxImpl) =>
+              or = nr /\
+              MinMaxSiR (fst nr) (snd nr)).
+    Focus 2.
+    unfold getObsDef; simpl; intros.
+
+
+    eapply SharpenStep with (adt' :=
                                {|
      Rep := Rep MinPlusMaxSpec * Rep MinMaxImpl;
      MutatorMethods := fun
@@ -69,13 +220,13 @@ Section MinMaxExample.
                          (r : Rep MinPlusMaxSpec * Rep MinMaxImpl)
                          (x : MutatorDom
                                 (CombTwoOpCollectionSig "MinPlusMax") idx) =>
-                       r1 <- MutatorMethods MinPlusMaxSpec idx (fst r) x;
-                       r2 <- MutatorMethods MinMaxImpl idx (snd r) x;
+                        r1 <- MutatorMethods MinPlusMaxSpec idx (fst r) x;
+     r2 <- MutatorMethods MinMaxImpl idx (snd r) x;
                        ret (r1, r2);
      ObserverMethods := fun
                           (idx : ObserverIndex
                                    (CombTwoOpCollectionSig "MinPlusMax"))
-                          (r : Rep MinPlusMaxSpec * Rep MinMaxImpl) 
+                          (r : Rep MinPlusMaxSpec * Rep MinMaxImpl)
                           n =>
                          (min <- (ObserverMethods MinMaxImpl
                                                   {|bounded_s := "Min"%string |} (snd r) (foo _ n));
@@ -91,17 +242,17 @@ Section MinMaxExample.
                                  (MutatorMethods MinMaxImpl idx))).
     inversion refineMinMax; eauto.
     clear refineMinMax; destruct H as [SiR [refineMinMaxObs refineMinMaxMut] ].
-    eapply refineADT_Build_ADT_Rep with 
-    (SiR := fun (or nr : Rep MinPlusMaxSpec * Rep MinMaxImpl) => 
+    eapply refineADT_Build_ADT_Rep with
+    (SiR := fun (or nr : Rep MinPlusMaxSpec * Rep MinMaxImpl) =>
               or = nr /\
               SiR (fst nr) (snd nr)).
     - intro.
       assert (exists pf,
                 mutIdx = {| bounded_s := "Insert"%string;
-                            s_bounded := pf |}) as mutIdx_eq by 
+                            s_bounded := pf |}) as mutIdx_eq by
           (clear;
-           destruct mutIdx; destruct s_bounded; inversion sbound; 
-           subst; simpl; 
+           destruct mutIdx; destruct s_bounded; inversion sbound;
+           subst; simpl;
            [ exists {| sbound := sbound |}; reflexivity
                   | inversion H ]) ;
       destruct mutIdx_eq as [pf mutIdx_eq]; rewrite mutIdx_eq.
@@ -114,17 +265,17 @@ Section MinMaxExample.
       unfold getMutDef in H0, H3; simpl in H0, H3.
       inversion_by computes_to_inv.
       unfold add_spec in *.
-      assert (x1 = x) by 
+      assert (x1 = x) by
           (apply functional_extensionality;
            intros; rewrite H0, H3; reflexivity).
       rewrite H in H4; assumption.
-    - intro; 
+    - intro;
       assert (exists pf,
                  obsIdx = {| bounded_s := "MinPlusMax"%string;
-                            s_bounded := pf |}) as obsIdx_eq by 
+                            s_bounded := pf |}) as obsIdx_eq by
           (clear;
-           destruct obsIdx; destruct s_bounded; inversion sbound; 
-           subst; simpl; 
+           destruct obsIdx; destruct s_bounded; inversion sbound;
+           subst; simpl;
            [ exists {| sbound := sbound |}; reflexivity
                   | inversion H ]) ;
       destruct obsIdx_eq as [pf obsIdx_eq]; rewrite obsIdx_eq.
@@ -144,7 +295,7 @@ Section MinMaxExample.
   Defined.
 
   (* Show the term derived above as a sanity check. *)
-  Goal (forall b, ObserverMethods (proj1_sig (MinPlusMaxImpl 0)) 
+  Goal (forall b, ObserverMethods (proj1_sig (MinPlusMaxImpl 0))
                                  {| bounded_s := "MinPlusMax" |} = b).
     simpl.
   Abort.
