ADTRefinement/BuildADTSetoidMorphisms.v
@@ -1,0 +1,48 @@
+Require Import Common Computation ADT Ensembles.
+Require Export ADTRefinement.Core ADTRefinement.SetoidMorphisms.
+
+Generalizable All Variables.
+Set Implicit Arguments.
+
+Lemma refineADT_BuildADT_Rep mutSigs obsSigs oldRep newRep
+      (SiR : oldRep -> newRep -> Prop)
+: respectful_hetero _ _ _ _
+      (fun oldMuts newMuts =>
+         forall mutIdx,
+           @refineMutator oldRep newRep SiR
+                          _
+                          (getMutDef oldMuts mutIdx)
+                          (getMutDef newMuts mutIdx))
+      (fun x y => respectful_hetero _ _ _ _
+                    (fun oldObs newObs =>
+                       forall obsIdx,
+                         @refineObserver oldRep newRep SiR _ _
+                                         (getObsDef oldObs obsIdx)
+                                         (getObsDef newObs obsIdx))
+                    (fun obs obs' => refineADT))
+     (@BuildADT oldRep mutSigs obsSigs)
+     (@BuildADT newRep mutSigs obsSigs).
+ Proof.
+   unfold Proper, respectful_hetero; intros.
+   let A := match goal with |- refineADT ?A ?B => constr:(A) end in
+   let B := match goal with |- refineADT ?A ?B => constr:(B) end in
+   eapply (@refinesADT _ A B SiR);
+     unfold id, pointwise_relation in *; simpl in *; intros; eauto.
+ Qed.
+
+Add Parametric Morphism rep mutSigs obsSigs
+: (@BuildADT rep mutSigs obsSigs)
+    with signature
+    (fun oldMuts newMuts =>
+       forall mutIdx, @refineMutator _ _ eq _
+                                  (getMutDef oldMuts mutIdx)
+                                  (getMutDef newMuts mutIdx))
+      ==> (fun oldObs newObs =>
+             forall obsIdx, @refineObserver _ _ eq _ _
+                                         (getObsDef oldObs obsIdx)
+                                         (getObsDef newObs obsIdx))
+      ==> refineADT
+      as refineADT_BuildADT_Both.
+Proof.
+  intros; eapply refineADT_BuildADT_Rep; eauto; reflexivity.
+Qed.
